arch/riscv/machine.s.dfy
@@ -80,10 +80,6 @@ module rv_machine {
             case T6 => 31
         }
     }
-    function method bv64_to_2s_comp(val: int64): uint64
-    {
-        if val >= 0 then val else val + BASE_64
-    }
 
     // datatype uint64_raw = uint64_cons(
     //     lh: uint32, uh: uint32, full: uint64)
@@ -92,39 +88,6 @@ module rv_machine {
     //     && num.lh == dw_lh(num.full)
     //     && num.uh == dw_uh(num.full)
     //     witness *
-
-    datatype int64_raw = int64_cons(
-        lh: uint32, uh: uint32, full: int64)
-
-    type int64_view_t = num: int64_raw |
-        && num.lh == dw_lh(bv64_to_2s_comp(num.full))
-        && num.uh == dw_uh(bv64_to_2s_comp(num.full)) 
-        witness *
-
-    lemma lemma_int64_half_split(num: int64_view_t)
-        ensures num.lh + num.uh * BASE_32 == bv64_to_2s_comp(num.full);
-    {
-        dw_split_lemma(bv64_to_2s_comp(num.full));
-    }
-
-    predicate valid_int64_view(
-        num: int64_view_t,
-        lh: uint32, uh: uint32)
-    {
-        && lh == num.lh
-        && uh == num.uh
-    }
-    
-    lemma lemma_int64_negative_one(num: int64_view_t)
-        requires num.lh == BASE_32 - 1
-        requires num.uh == BASE_32 - 1
-        ensures num.full == -1
-    {
-        lemma_int64_half_split(num);
-        assert num.lh + num.uh * BASE_32 == bv64_to_2s_comp(num.full);
-        assert num.lh + num.uh * BASE_32 == BASE_64 - 1;
-        assert num.full == -1;
-    }
 
    /* memory definitions */ 
 
